commit

AP/System/Symmetry.lean
@@ -1,26 +1,5 @@
 import AP.System.Invariant
 
-namespace Equiv
-
-variable {α β γ : Type*}
-variable {e : α ≃ β} {e₁ : β ≃ γ} {e₂ : α ≃ β}
-
-def comp (e₁ : β ≃ γ) (e₂ : α ≃ β) : α ≃ γ where
-  toFun := e₁ ∘ e₂
-  invFun := e₂.symm ∘ e₁.symm
-  left_inv := by intros x; simp
-  right_inv := by intros x; simp
-
-@[simp]
-theorem coe_toFun_comp : (e₁.comp e₂ : _ → _) = e₁ ∘ e₂ := rfl
-
-@[simp]
-theorem symm_comp : (e₁.comp e₂).symm = e₂.symm.comp e₁.symm := rfl
-
--- #check 0 #exit
-
-end Equiv
-
 namespace System
 
 universe u
@@ -32,18 +11,18 @@ structure Symmetry (sys : System S T) : Type u where
   fs' : S → S
   ft : T → T
   ft' : T → T
+  h_fs : BijectiveOn sys.WF sys.WF fs fs'
+  h_ft : BijectiveOn sys.WFTrans sys.WFTrans ft ft'
+  tr_eq : ∀ {s t} [sys.WF s], sys.tr s t = (sys.tr (fs s) (ft t)).map fs'
+  tr_eq' : ∀ {s t} [sys.WF s], sys.tr s t = (sys.tr (fs' s) (ft' t)).map fs
 
 namespace Symmetry
 
 variable {sym sym₁ sym₂ : sys.Symmetry}
 
-class WF (sym : sys.Symmetry) : Prop where
-  h_fs : BijectiveOn sys.WF sys.WF sym.fs sym.fs'
-  h_ft : BijectiveOn sys.WFTrans sys.WFTrans sym.ft sym.ft'
-  tr_eq : ∀ {s t} [sys.WF s], sys.tr s t = (sys.tr (sym.fs s) (sym.ft t)).map sym.fs'
-  tr_eq' : ∀ {s t} [sys.WF s], sys.tr s t = (sys.tr (sym.fs' s) (sym.ft' t)).map sym.fs
-
-def one : sys.Symmetry := ⟨id, id, id, id⟩
+def one : sys.Symmetry where
+  fs := id; fs' := id; ft := id; ft' := id
+  h_fs := by simp;; h_ft := by simp;; tr_eq := by simp;; tr_eq' := by simp
 
 instance : One sys.Symmetry := ⟨one⟩
 theorem one_def : (1 : sys.Symmetry) = one := rfl
@@ -51,109 +30,101 @@ theorem one_def : (1 : sys.Symmetry) = one := rfl
 instance : Inhabited sys.Symmetry := ⟨one⟩
 theorem default_eq : (default : sys.Symmetry) = 1 := rfl
 
-@[simp]
-instance : (1 : sys.Symmetry).WF := by
-  rw [one_def, one]; constructor <;> simp
+instance {s} [hs : sys.WF s] : sys.WF (sym.fs s) :=
+  sym.h_fs.cnd_right hs
+
+instance {s} [hs : sys.WF s] : sys.WF (sym.fs' s) :=
+  sym.h_fs.cnd_left hs
+
+instance {t} [ht : sys.WFTrans t] : sys.WFTrans (sym.ft t) :=
+  sym.h_ft.cnd_right ht
+
+instance {t} [ht : sys.WFTrans t] : sys.WFTrans (sym.ft' t) :=
+  sym.h_ft.cnd_left ht
 
 @[simp]
-instance : (default : sys.Symmetry).WF := by
-  rw [default_eq]; infer_instance
-
-instance {s} [H : sym.WF] [hs : sys.WF s] : sys.WF (sym.fs s) :=
-  H.h_fs.cnd_right hs
-
-instance {s} [H : sym.WF] [hs : sys.WF s] : sys.WF (sym.fs' s) :=
-  H.h_fs.cnd_left hs
-
-instance {t} [H : sym.WF] [ht : sys.WFTrans t] : sys.WFTrans (sym.ft t) :=
-  H.h_ft.cnd_right ht
-
-instance {t} [H : sym.WF] [ht : sys.WFTrans t] : sys.WFTrans (sym.ft' t) :=
-  H.h_ft.cnd_left ht
+theorem fs'_fs {s} [hs : sys.WF s] : sym.fs' (sym.fs s) = s :=
+  sym.h_fs.cancel_left hs
 
 @[simp]
-theorem fs'_fs {s} [H : sym.WF] [hs : sys.WF s] : sym.fs' (sym.fs s) = s :=
-  H.h_fs.cancel_left hs
+theorem fs_fs' {s} [hs : sys.WF s] : sym.fs (sym.fs' s) = s :=
+  sym.h_fs.cancel_right hs
 
 @[simp]
-theorem fs_fs' {s} [H : sym.WF] [hs : sys.WF s] : sym.fs (sym.fs' s) = s :=
-  H.h_fs.cancel_right hs
+theorem ft'_ft {t} [ht : sys.WFTrans t] : sym.ft' (sym.ft t) = t :=
+  sym.h_ft.cancel_left ht
 
 @[simp]
-theorem ft'_ft {t} [H : sym.WF] [ht : sys.WFTrans t] : sym.ft' (sym.ft t) = t :=
-  H.h_ft.cancel_left ht
+theorem ft_ft' {t} [ht : sys.WFTrans t] : sym.ft (sym.ft' t) = t :=
+  sym.h_ft.cancel_right ht
 
-@[simp]
-theorem ft_ft' {t} [H : sym.WF] [ht : sys.WFTrans t] : sym.ft (sym.ft' t) = t :=
-  H.h_ft.cancel_right ht
-
-def tr_fs {s t} [H : sym.WF] [hs : sys.WF s] :
+def tr_fs {s t} [hs : sys.WF s] :
 sys.tr (sym.fs s) t = (sys.tr s (sym.ft' t)).map sym.fs := by
-  nth_rw 1 [H.tr_eq']; ext s'; simp
+  nth_rw 1 [sym.tr_eq']; ext s'; simp
 
-def tr_fs' {s t} [H : sym.WF] [hs : sys.WF s] :
+def tr_fs' {s t} [hs : sys.WF s] :
 sys.tr (sym.fs' s) t = (sys.tr s (sym.ft t)).map sym.fs' := by
-  nth_rw 1 [H.tr_eq]; ext s'; simp
+  nth_rw 1 [sym.tr_eq]; ext s'; simp
 
-def tr_ft {s t} [H : sym.WF] [hs : sys.WF s] :
+def tr_ft {s t} [hs : sys.WF s] :
 sys.tr s (sym.ft t) = (sys.tr (sym.fs' s) t).map sym.fs := by
-  nth_rw 2 [H.tr_eq]; ext s'; simp; constructor
+  nth_rw 2 [sym.tr_eq]; ext s'; simp; constructor
   · intro h; use s'; have hs' := wf_of_tr h; simpa
   · rintro ⟨s₁, h₁, h₂⟩; have hs₁ := wf_of_tr h₁; simp at h₂; simpa [←h₂]
 
-def tr_ft' {s t} [H : sym.WF] [hs : sys.WF s] :
+def tr_ft' {s t} [hs : sys.WF s] :
 sys.tr s (sym.ft' t) = (sys.tr (sym.fs s) t).map sym.fs' := by
-  nth_rw 2 [H.tr_eq']; ext s'; simp; constructor
+  nth_rw 2 [sym.tr_eq']; ext s'; simp; constructor
   · intro h; use s', h; have h₁ := wf_of_tr h; simp
   · rintro ⟨s₁, h₁, h₂⟩; have h₃ := wf_of_tr h₁; simp at h₂; simpa [←h₂]
 
-theorem validTr_fs_of {s t} [H : sym.WF] [hs : sys.WF s]
+theorem validTr_fs_of {s t} [hs : sys.WF s]
 (h : sys.validTr s (sym.ft' t)) : sys.validTr (sym.fs s) t := by
   obtain ⟨s', h⟩ := h; simp [tr_ft'] at h; obtain ⟨s', h, rfl⟩ := h; use s'
 
-theorem validTr_fs'_of {s t} [H : sym.WF] [hs : sys.WF s]
+theorem validTr_fs'_of {s t} [hs : sys.WF s]
 (h : sys.validTr s (sym.ft t)) : sys.validTr (sym.fs' s) t := by
   obtain ⟨s', h⟩ := h; simp [tr_ft] at h; obtain ⟨s', h, rfl⟩ := h; use s'
 
-theorem validTr_ft_of {s t} [H : sym.WF] [hs : sys.WF s]
+theorem validTr_ft_of {s t} [hs : sys.WF s]
 (h : sys.validTr (sym.fs' s) t) : sys.validTr s (sym.ft t) := by
   obtain ⟨s', h⟩ := h; simp [tr_fs'] at h; obtain ⟨s', h, rfl⟩ := h; use s'
 
-theorem validTr_ft'_of {s t} [H : sym.WF] [hs : sys.WF s]
+theorem validTr_ft'_of {s t} [hs : sys.WF s]
 (h : sys.validTr (sym.fs s) t) : sys.validTr s (sym.ft' t) := by
   obtain ⟨s', h⟩ := h; simp [tr_fs] at h; obtain ⟨s', h, rfl⟩ := h; use s'
 
-theorem validTr_fs {s t} [H : sym.WF] [hs : sys.WF s] :
+theorem validTr_fs {s t} [hs : sys.WF s] :
 sys.validTr (sym.fs s) t ↔ sys.validTr s (sym.ft' t) :=
   ⟨validTr_ft'_of, validTr_fs_of⟩
 
-theorem validTr_fs' {s t} [H : sym.WF] [hs : sys.WF s] :
+theorem validTr_fs' {s t} [hs : sys.WF s] :
 sys.validTr (sym.fs' s) t ↔ sys.validTr s (sym.ft t) :=
   ⟨validTr_ft_of, validTr_fs'_of⟩
 
-theorem validTr_ft {s t} [H : sym.WF] [hs : sys.WF s] :
+theorem validTr_ft {s t} [hs : sys.WF s] :
 sys.validTr s (sym.ft t) ↔ sys.validTr (sym.fs' s) t :=
   ⟨validTr_fs'_of, validTr_ft_of⟩
 
-theorem validTr_ft' {s t} [H : sym.WF] [hs : sys.WF s] :
+theorem validTr_ft' {s t} [hs : sys.WF s] :
 sys.validTr s (sym.ft' t) ↔ sys.validTr (sym.fs s) t :=
   ⟨validTr_fs_of, validTr_ft'_of⟩
 
 @[simp]
-theorem hasTr_fs {s} [H : sym.WF] [hs : sys.WF s] :
+theorem hasTr_fs {s} [hs : sys.WF s] :
 sys.hasTr (sym.fs s) ↔ sys.hasTr s := by
   constructor <;> rintro ⟨t, h⟩
   · use sym.ft' t; simpa [validTr_ft']
   · use sym.ft t; simpa [validTr_ft]
 
 @[simp]
-theorem hasTr_fs' {s} [H : sym.WF] [hs : sys.WF s] :
+theorem hasTr_fs' {s} [hs : sys.WF s] :
 sys.hasTr (sym.fs' s) ↔ sys.hasTr s := by
   constructor <;> rintro ⟨t, h⟩
   · use sym.ft t; simpa [validTr_ft]
   · use sym.ft' t; simpa [validTr_ft']
 
-example {s t} [H : sym.WF] [hs : sys.WF s] :
+example {s t} [hs : sys.WF s] :
 sys.validTr (sym.fs s) t ↔ sys.validTr s (sym.ft' t) := by
   symm; constructor
   · exact fun a ↦ validTr_fs_of a
@@ -163,7 +134,7 @@ sys.validTr (sym.fs s) t ↔ sys.validTr s (sym.ft' t) := by
 def simFn (sym : sys.Symmetry) (f : S → T) (s : S) : T :=
   sym.ft # f # sym.fs' s
 
-instance {f} [H : sym.WF] [hf : sys.SimFn f] : sys.SimFn (sym.simFn f) := by
+instance {f} [hf : sys.SimFn f] : sys.SimFn (sym.simFn f) := by
   rw [sys.simFn_def]; intro s hs h; simp; apply hf.1 at h; apply validTr_ft_of
   have h₁ : sys.hasTr (sym.fs' s); simp; exact ⟨_, h⟩; exact hf.1 h₁
 
@@ -172,6 +143,10 @@ def inv (sym : sys.Symmetry) : sys.Symmetry where
   fs' := sym.fs
   ft' := sym.ft
   ft := sym.ft'
+  h_fs := sym.h_fs.symm
+  h_ft := sym.h_ft.symm
+  tr_eq := sym.tr_eq'
+  tr_eq' := sym.tr_eq
 
 instance : Inv sys.Symmetry := ⟨.inv⟩
 theorem inv_def : sym⁻¹ = sym.inv := rfl
@@ -179,57 +154,42 @@ theorem inv_def : sym⁻¹ = sym.inv := rfl
 @[simp]
 protected theorem inv_inv : sym⁻¹⁻¹ = sym := by ext <;> rfl
 
-instance [H : sym.WF] : sym⁻¹.WF where
-  h_fs := H.h_fs.symm
-  h_ft := H.h_ft.symm
-  tr_eq := WF.tr_eq'
-  tr_eq' := WF.tr_eq
-
-@[simp]
-theorem wf_inv_iff : sym⁻¹.WF ↔ sym.WF := by
-  symm; constructor <;> intro h; infer_instance
-  rw [←sym.inv_inv]; infer_instance
-
 def mul (sym₁ sym₂ : sys.Symmetry) : sys.Symmetry where
   fs := sym₁.fs ∘ sym₂.fs
   fs' := sym₂.fs' ∘ sym₁.fs'
   ft := sym₁.ft ∘ sym₂.ft
   ft' := sym₂.ft' ∘ sym₁.ft'
-
-instance : Mul sys.Symmetry := ⟨mul⟩
-theorem mul_def : sym₁ * sym₂ = sym₁.mul sym₂ := rfl
-
-@[simp]
-instance [H₁ : sym₁.WF] [H₂ : sym₂.WF] : (sym₁ * sym₂).WF := by
-  rw [mul_def, mul]; constructor <;> dsimp
-  · constructor; have ⟨e₁, h₁, h₂⟩ := H₁.h_fs; have ⟨e₂, h₃, h₄⟩ := H₂.h_fs
+  h_fs := by
+    constructor; have ⟨e₁, h₁, h₂⟩ := sym₁.h_fs; have ⟨e₂, h₃, h₄⟩ := sym₂.h_fs
     use e₁.comp e₂; constructor <;> intro s hs <;> simp
     rw [h₃ hs]; apply h₁; rw [h₂ hs]; apply h₄
-  · constructor; have ⟨e₁, h₁, h₂⟩ := H₁.h_ft; have ⟨e₂, h₃, h₄⟩ := H₂.h_ft
+  h_ft := by
+    constructor; have ⟨e₁, h₁, h₂⟩ := sym₁.h_ft; have ⟨e₂, h₃, h₄⟩ := sym₂.h_ft
     use e₁.comp e₂; constructor <;> intro s hs <;> simp
     rw [h₃ hs]; apply h₁; rw [h₂ hs]; apply h₄
-  · intro s t hs; ext s'; simp; constructor
+  tr_eq := by
+    intro s t hs; ext s'; simp; constructor
     · intro h₁; have hs' := wf_of_tr h₁; use sym₁.fs # sym₂.fs s'
       have ht := wfTrans_of_tr h₁; simp [tr_fs]; use s'
     · rintro ⟨s', h₁, rfl⟩; have hs₁ := wf_of_tr h₁; simp [tr_ft] at h₁
       obtain ⟨s', h₁, rfl⟩ := h₁; have hs' := wf_of_tr h₁; simpa
-  · intro s t hs; ext s'; simp; constructor
+  tr_eq' := by
+    intro s t hs; ext s'; simp; constructor
     · intro h₁; have hs' := wf_of_tr h₁; use sym₂.fs' # sym₁.fs' s'
       have ht := wfTrans_of_tr h₁; simp [tr_fs']; use s'
     · rintro ⟨s', h₁, rfl⟩; have hs₁ := wf_of_tr h₁; simp [tr_ft'] at h₁
       obtain ⟨s', h₁, rfl⟩ := h₁; have hs' := wf_of_tr h₁; simpa
 
+instance : Mul sys.Symmetry := ⟨mul⟩
+theorem mul_def : sym₁ * sym₂ = sym₁.mul sym₂ := rfl
+
 def npow (n : ℕ) (sym : sys.Symmetry) : sys.Symmetry :=
   (· * sym)^[n] 1
 
-protected theorem one_mul : 1 * sym = sym := rfl
-protected theorem mul_one : sym * 1 = sym := rfl
-protected theorem mul_assoc {s₁ s₂ s₃ : sys.Symmetry} : s₁ * s₂ * s₃ = s₁ * (s₂ * s₃) := rfl
-
 instance : Monoid sys.Symmetry where
-  one_mul := λ _ => Symmetry.one_mul
-  mul_one := λ _ => Symmetry.mul_one
-  mul_assoc := λ _ _ _ => Symmetry.mul_assoc
+  one_mul := λ _ => rfl
+  mul_one := λ _ => rfl
+  mul_assoc := λ _ _ _ => rfl
   npow := npow
   npow_succ := by intros; simp_rw [npow, Function.iterate_succ']; simp
 
@@ -247,6 +207,7 @@ protected theorem inv_mul_cancel : sym * sym⁻¹ = 1 := by
   ext
   · nm s
     simp [inv_def, mul_def, one_def, inv, mul, one]
+    simp
 
 #check 0 #exit
 
